lean/src/a_eval_theorem.lean
@@ -5,13 +5,6 @@ import .lemmas
 variable [GuardModule]
 open GuardModule
 
-lemma foo (ant: Ant Φ) (ty: Φ) (env: Env):
-    ant_eval (map_ant (ty.and) ant) env
-    = ant_eval' (map_ant (band (Φ_eval ty env)) (ant_eval_all ant env)) :=
-begin
-    sorry
-end
-
 attribute [simp]
 lemma ant_eval'_simp1 (r: option Result) :
     ant_eval'._match_1 (some Result.no_match, r) = r :=
@@ -45,15 +38,30 @@ begin
     finish,    
 end
 
-
-local attribute [simp] ant_eval ant_eval_all map_ant ant_eval' Φ_eval
-
-lemma and_no_match (ant: Ant Φ) (ty: Φ) (env: Env):
-    ant_eval ant env = some Result.no_match
-    → ant_eval (map_ant (ty.and) ant) env = some Result.no_match :=
+attribute [simp]
+lemma ant_eval'_simp4 (r: option Result) :
+    ant_eval'._match_2 (ff, r) = r :=
 begin
-    assume h,
-    
+    cases r;
+    try { cases r };
+    finish,
+end
+
+attribute [simp]
+lemma ant_eval'_simp5 (r: option Result) (h: r ≠ some Result.no_match) :
+    ant_eval'._match_2 (tt, r) = none :=
+begin
+    cases r;
+    try { cases r };
+    finish,
+end
+
+
+local attribute [simp] 𝒜' ant_eval ant_eval_all map_ant ant_eval' Φ_eval gdt_eval 
+
+lemma and_no_match (ant: Ant Φ) (ty: Φ) (env: Env) (h: ant_eval ant env = some Result.no_match):
+    ant_eval (map_ant (ty.and) ant) env = some Result.no_match :=
+begin
     induction ant,
 
     case Ant.leaf {
@@ -72,13 +80,8 @@ begin
     },
 
     case Ant.diverge {
-        simp at h,
-        simp,
-
-        rw ←ant_eval_all,
-        rw ←ant_eval,
-        rw ←ant_eval_all at h,
-        rw ←ant_eval at h,
+        simp at h, rw [←ant_eval_all, ←ant_eval] at h,
+        simp, rw [←ant_eval_all, ←ant_eval],
 
         have z : Φ_eval ant_a env = ff ∧ ant_eval ant_tr env = some Result.no_match, {
             cases Φ_eval ant_a env;
@@ -94,28 +97,22 @@ end
 
 
 
-lemma ant_eval_is_some_and (ant: Ant Φ) (env: Env) (ty: Φ):
-    option.is_some (ant_eval ant env)
-    → option.is_some (ant_eval (map_ant (ty.and) ant) env) :=
+lemma ant_eval_is_some_and (ant: Ant Φ) (env: Env) (ty: Φ) (h: option.is_some (ant_eval ant env)):
+    option.is_some (ant_eval (map_ant (ty.and) ant) env) :=
 begin
-    assume h,
     induction ant with h2,
     
-        
-    
+
     case Ant.leaf {
-        unfold 𝒜' map_ant ant_eval ant_eval ant_eval_all map_ant ant_eval',
-        cases Φ_eval (ty.and h2) env,
-        all_goals { simp },
+        simp,
+        by_cases ↥(Φ_eval ty env) ∧ ↥(Φ_eval h2 env);
+        finish,
     },
 
     case Ant.branch {
         
         conv at h {
-            rw ant_eval,
-            rw ant_eval_all,
-            rw map_ant,
-            rw ant_eval',
+            simp,
             rw ← ant_eval_all,
             rw ← ant_eval_all,
             rw ←ant_eval,
@@ -123,66 +120,83 @@ begin
         },
 
         conv {
-            rw map_ant,
-            rw ant_eval,
-            rw ant_eval_all,
-            rw map_ant,
-            rw ant_eval',
-            rw ← ant_eval_all,
+            simp,
             rw ← ant_eval_all,
             rw ←ant_eval,
+            rw ← ant_eval_all,
             rw ←ant_eval,
         },
         
+        by_cases h_1: (ant_eval ant_tr1 env = some Result.no_match);
+        by_cases h_2: (ant_eval ant_tr2 env = some Result.no_match),
         
-        by_cases h_1: (ant_eval ant_tr1 env = some Result.no_match),
-        all_goals {
-            by_cases h_2: (ant_eval ant_tr2 env = some Result.no_match),
+        {
+            rw (and_no_match _ _ _ h_1),
+            rw (and_no_match _ _ _ h_2),
+            simp,
         },
         {
-            rw h_1 at ant_ih_tr1,
-            simp at ant_ih_tr1,
-            rw h_2 at ant_ih_tr2,
-            simp at ant_ih_tr2,
-            rw and_no_match,
-            rw and_no_match,
-            rw ant_eval'._match_1,
-            simp,
-            exact h_2,
+            rw (and_no_match _ _ _ h_1),
+            rw ant_eval'_simp1,
+            rw h_1 at h,
+            rw ant_eval'_simp1 at h,
+            exact ant_ih_tr2 h,
+        },
+        {
+            rw (and_no_match _ _ _ h_2),
+            rw ant_eval'_simp2,
+            rw h_2 at h,
+            rw ant_eval'_simp2 at h,
+            exact ant_ih_tr1 h,
+        },
+        {
+            rw ant_eval'_simp3 at h,
+            simp at h,
+            contradiction,
             exact h_1,
+            exact h_2,
         },
-        
-        
+    },
+
+    case Ant.diverge {
+        simp,
+        rw ← ant_eval_all,
+        rw ←ant_eval,
+
+        simp at h,
+        rw ← ant_eval_all at h,
+        rw ←ant_eval at h,
 
 
-        /-
-        conv in (ant_eval (map_ant ty.and (𝒜' (gdt_tr1.branch gdt_tr2))) env).is_some {
-            rw 𝒜',
-            rw map_ant,
-            rw ant_eval,
-            rw ant_eval_all,
-            rw map_ant,
-            rw ant_eval',
-            rw ← ant_eval_all,
+        cases Φ_eval ant_a env;
+        by_cases x: ant_eval ant_tr env = some Result.no_match,
+        all_goals {
+            simp,
             rw ← ant_eval_all,
             rw ←ant_eval,
-            rw ←ant_eval,
         },
-        -/
-        
-        
-        /-
-        rw map_ant at h,
-        rw ← ant_eval_all at h,
-        rw ← ant_eval_all at h,
 
-        rw ant_eval' at h,
-        rw ←ant_eval at h,
-        rw ←ant_eval at h,
-        
-        rw map_ant at h,
-        rw ant_eval' at h,
-        -/
+        {
+            rw and_no_match _ _ _ x,
+            simp,
+        },
+        {
+            simp at h,
+            rw ← ant_eval_all at h,
+            rw ←ant_eval at h,
+            exact ant_ih h,
+        },
+        {
+            rw and_no_match _ _ _ x,
+            cases Φ_eval ty env;
+            simp,
+        },
+        {
+            rw ant_eval'_simp5 at h,
+            simp at h,
+            contradiction,
+            exact x,
+        },
     },
 end
 
@@ -205,27 +219,127 @@ begin
     },
 
     case Gdt.branch {
-        unfold 𝒜',
-        unfold ant_eval,
-        unfold ant_eval_all,
-        unfold map_ant,
-        rw ←ant_eval_all,
-        rw ←ant_eval_all,
-        unfold ant_eval',
-        rw ←ant_eval,
-        rw ←ant_eval,
-        rw ←gdt_ih_tr1,
+        simp,
+        rw [←ant_eval_all, ←ant_eval],
+        rw [←ant_eval_all, ←ant_eval],
+        
+
+
+/-
+    gdt_ih_tr1: some (gdt_eval gdt_tr1 env) = ant_eval (𝒜' gdt_tr1) env
+    gdt_ih_tr2: some (gdt_eval gdt_tr2 env) = ant_eval (𝒜' gdt_tr2) env
+
+        some (
+            gdt_eval._match_1
+                (gdt_eval gdt_tr2 env)
+                (gdt_eval gdt_tr1 env)
+        )
+        
+        = ant_eval'._match_1
+            (
+                ant_eval (𝒜' gdt_tr1) env,
+                ant_eval (map_ant (𝒰' gdt_tr1).and (𝒜' gdt_tr2)) env
+            )
+
+
+
+
+
+
+
+
+
+
+
+
+
+
+
+    gdt_ih_tr1: some (gdt_eval gdt_tr1 env) = ant_eval (𝒜' gdt_tr1) env
+    gdt_ih_tr2: some (gdt_eval gdt_tr2 env) = ant_eval (𝒜' gdt_tr2) env
+
+        some (
+            match gdt_eval gdt_tr1 env with
+            | Result.no_match := gdt_eval gdt_tr2 env
+            | r := r
+            end
+        )
+        =
+            match (ant_eval (𝒜' gdt_tr1) env, ant_eval (map_ant (𝒰' gdt_tr1).and (𝒜' gdt_tr2)) env) with
+            | (some Result.no_match, r) := r
+            | (r, some Result.no_match) := r
+            | _ := none
+            end
+
+
+
+
+
+
+
+
+
+
+
+
+
+
+
+
+
+    gdt_ih_tr1: some (gdt_eval gdt_tr1 env) = ant_eval (𝒜' gdt_tr1) env
+    gdt_ih_tr2: some (gdt_eval gdt_tr2 env) = ant_eval (𝒜' gdt_tr2) env
+
+        some (
+            match gdt_eval gdt_tr1 env with
+                | Result.no_match := gdt_eval gdt_tr2 env
+                | r := r
+            end
+        )
+        =
+            match (
+                some (gdt_eval gdt_tr1 env),
+                ant_eval (map_ant (𝒰' gdt_tr1).and (𝒜' gdt_tr2)) env
+            ) with
+                | (some Result.no_match, r) := r
+                | (r, some Result.no_match) := r
+                | _ := none
+            end
+
+
+
+
+-/
 
 
         cases c: (ant_eval (map_ant (𝒰' gdt_tr1).and (𝒜' gdt_tr2)) env),
 
         case option.none {
-
+            have x: (option.is_some (ant_eval (𝒜' gdt_tr2) env) : Prop) := begin
+                rw ←gdt_ih_tr2,
+                simp,
+            end,
+            let q := (ant_eval_is_some_and _ _ _ x), 
+            rw c at q,
+            simp at q,
+            contradiction,
         },
 
 
 
+        rw ←gdt_ih_tr1,
 
+
+
+
+
+
+
+
+
+
+
+        
 
         cases (gdt_eval gdt_tr1 env),
         all_goals {
